Seal iProp primitives

theories/IPM.v
@@ -13,36 +13,76 @@ Set Implicit Arguments.
 Set Typeclasses Depth 5.
 
 
+Create HintDb iprop.
 
 Section IRIS.
   Context {Σ: GRA.t}.
   Definition iProp := Σ -> Prop.
 
   Definition Sepconj (P Q: iProp): iProp :=
-    fun r => exists a b, r = URA.add a b /\ P a /\ Q b
-  .
-  Definition Pure (P: Prop): iProp := fun _ => P.
-  Definition Ex {X: Type} (P: X -> iProp): iProp := fun r => exists x, P x r.
-  Definition Univ {X: Type} (P: X -> iProp): iProp := fun r => forall x, P x r.
-  Definition Own (r0: Σ): iProp := fun r1 => URA.extends r0 r1.
-  Definition And (P Q: iProp): iProp := fun r => P r /\ Q r.
-  Definition Or (P Q: iProp): iProp := fun r => P r \/ Q r.
-  Definition Impl (P Q: iProp): iProp := fun r => URA.wf r -> P r -> Q r.
-  Definition Wand (P Q: iProp): iProp := fun r => forall rp, URA.wf (r ⋅ rp) -> P rp -> Q (r ⋅ rp).
+    Seal.sealing
+      "iProp"
+      (fun r => exists a b, r = URA.add a b /\ P a /\ Q b).
+  Definition Pure (P: Prop): iProp :=
+    Seal.sealing
+      "iProp"
+      (fun _ => P).
+  Definition Ex {X: Type} (P: X -> iProp): iProp :=
+    Seal.sealing
+      "iProp"
+      (fun r => exists x, P x r).
+  Definition Univ {X: Type} (P: X -> iProp): iProp :=
+    Seal.sealing
+      "iProp"
+      (fun r => forall x, P x r).
+  Definition Own (r0: Σ): iProp :=
+    Seal.sealing
+      "iProp"
+      (fun r1 => URA.extends r0 r1).
+  Definition And (P Q: iProp): iProp :=
+    Seal.sealing
+      "iProp"
+      (fun r => P r /\ Q r).
+  Definition Or (P Q: iProp): iProp :=
+    Seal.sealing
+      "iProp"
+      (fun r => P r \/ Q r).
+  Definition Impl (P Q: iProp): iProp :=
+    Seal.sealing
+      "iProp"
+      (fun r => URA.wf r -> P r -> Q r).
+  Definition Wand (P Q: iProp): iProp :=
+    Seal.sealing
+      "iProp"
+      (fun r => forall rp, URA.wf (r ⋅ rp) -> P rp -> Q (r ⋅ rp)).
+  Definition Emp: iProp :=
+    Seal.sealing
+      "iProp"
+      (eq ε).
+  Definition Persistently (P: iProp): iProp :=
+    Seal.sealing
+      "iProp"
+      (Pure (P ε)).
+  Definition Later (P: iProp): iProp :=
+    Seal.sealing
+      "iProp"
+      P.
+  Definition Upd (P: iProp): iProp :=
+    Seal.sealing
+      "iProp"
+      (fun r0 => forall ctx, URA.wf (r0 ⋅ ctx) -> exists r1, URA.wf (r1 ⋅ ctx) /\ P r1).
 
-  Definition Entails2 (P Q : iProp) : Prop :=
-    Seal.sealing "iProp" (forall r (WF: URA.wf r), P r -> Q r).
+  Definition Entails (P Q : iProp) : Prop :=
+    Seal.sealing
+      "iProp"
+      (forall r (WF: URA.wf r), P r -> Q r).
 
-  Inductive Entails (P Q : iProp) : Prop :=
-    { iProp_entails :> forall r (WF: URA.wf r), P r -> Q r }.
+  Hint Rewrite (Seal.sealing_eq "iProp"): iprop.
+  #[local] Hint Unfold Sepconj Pure Ex Univ Own And Or Impl Wand Emp Persistently Later Upd Entails: iprop.
 
-  (* Definition Entails (P Q: iProp): Prop := forall r (WF: URA.wf r), P r -> Q r. *)
-
-  Definition Upd (P: iProp): iProp := fun r0 => forall ctx, URA.wf (r0 ⋅ ctx) -> exists r1, URA.wf (r1 ⋅ ctx) /\ P r1.
-
-  Definition Emp: iProp := eq ε.
-  Definition Persistently (P: iProp): iProp := Pure (P ε).
-  Definition Later (P: iProp): iProp := P.
+  Ltac uipropall :=
+    autounfold with iprop; autorewrite with iprop;
+    all_once_fast ltac:(fun H => autounfold with iprop in H; autorewrite with iprop in H).
 
   (* Trivial Ofe Structure *)
   Inductive uPred_equiv' (P Q : iProp) : Prop :=
@@ -80,142 +120,142 @@ Section IRIS.
   Global Program Instance PreOrder_Entails: PreOrder Entails.
   Next Obligation.
   Proof.
-    ii. ss.
+    ii. uipropall. ss.
   Qed.
   Next Obligation.
   Proof.
-    ii. econs. ii. exploit (H r); et. eapply H0. auto.
+    ii. uipropall. ii. exploit (H r); et.
   Qed.
 
   Lemma Pure_intro: ∀ (φ : Prop) (P : iProp), φ → Entails P (Pure φ).
   Proof.
-    ii. ss.
+    ii. uipropall. ss.
   Qed.
 
   Lemma Pure_elim: ∀ (φ : Prop) (P : iProp), (φ → Entails (Pure True) P) → Entails (Pure φ) P.
   Proof.
-    ii. econs. ii. eapply H in H0. eapply H0; ss.
+    ii. uipropall. ii. eapply H in H0; et.
   Qed.
 
   Lemma And_elim_l: ∀ P Q : iProp, Entails (And P Q) P.
   Proof.
-    ii. econs. ii. eapply H.
+    ii. uipropall. ii. eapply H.
   Qed.
 
   Lemma And_elim_r: ∀ P Q : iProp, Entails (And P Q) Q.
   Proof.
-    ii. econs. ii. eapply H.
+    ii. uipropall. ii. eapply H.
   Qed.
 
   Lemma And_intro: ∀ P Q R : iProp, Entails P Q → Entails P R → Entails P (And Q R).
   Proof.
-    ii. econs. ii. split; [eapply H|eapply H0]; et.
+    ii. uipropall. ii. split; [eapply H|eapply H0]; et.
   Qed.
 
   Lemma Or_intro_l: ∀ P Q : iProp, Entails P (Or P Q).
   Proof.
-    ii. econs. ii. left. ss.
+    ii. uipropall. ii. left. ss.
   Qed.
 
   Lemma Or_intro_r: ∀ P Q : iProp, Entails Q (Or P Q).
   Proof.
-    ii. econs. ii. right. ss.
+    ii. uipropall. ii. right. ss.
   Qed.
 
   Lemma Or_elim: ∀ P Q R : iProp, Entails P R → Entails Q R → Entails (Or P Q) R.
   Proof.
-    ii. econs. ii. inv H1.
+    ii. uipropall. ii. inv H1.
     { eapply H; ss. }
     { eapply H0; ss. }
   Qed.
 
   Lemma Impl_intro_r: ∀ P Q R : iProp, Entails (And P Q) R → Entails P (Impl Q R).
   Proof.
-    ii. econs. ii. eapply H; et. split; ss.
+    ii. uipropall. ii. eapply H; et.
   Qed.
 
   Lemma Impl_elim_l: ∀ P Q R : iProp, Entails P (Impl Q R) → Entails (And P Q) R.
   Proof.
-    ii. econs. ii. inv H0. eapply H; et.
+    ii. uipropall. ii. inv H0. eapply H; et.
   Qed.
 
   Lemma Univ_intro: ∀ (A : Type) (P : iProp) (Ψ : A → iProp), (∀ a : A, Entails P (Ψ a)) → Entails P (Univ (λ a : A, Ψ a)).
   Proof.
-    ii. econs. ii. eapply H; et.
+    ii. uipropall. ii. specialize (H x). uipropall. eapply H; et.
   Qed.
 
   Lemma Univ_elim: ∀ (A : Type) (Ψ : A → iProp) (a : A), Entails (Univ (λ a0 : A, Ψ a0)) (Ψ a).
   Proof.
-    ii. econs. ii. eapply H; et.
+    ii. uipropall. ii. eapply H; et.
   Qed.
 
   Lemma Ex_intro: ∀ (A : Type) (Ψ : A → iProp) (a : A), Entails (Ψ a) (Ex (λ a0 : A, Ψ a0)).
   Proof.
-    ii. econs. ii. eexists. eauto.
+    ii. uipropall. ii. eexists. eauto.
   Qed.
 
   Lemma Ex_elim: ∀ (A : Type) (Φ : A → iProp) (Q : iProp), (∀ a : A, Entails (Φ a) Q) → Entails (Ex (λ a : A, Φ a)) Q.
   Proof.
-    ii. econs. ii. inv H0. eapply H; et.
+    ii. uipropall. ii. des. specialize (H x). uipropall. et.
   Qed.
 
   Lemma Sepconj_mono: ∀ P P' Q Q' : iProp, Entails P Q → Entails P' Q' → Entails (Sepconj P P') (Sepconj Q Q').
   Proof.
-    ii. econs. ii. unfold Sepconj in *. des; subst. esplits; et.
+    ii. uipropall. ii. unfold Sepconj in *. des; subst. esplits; et.
     { eapply H; et. eapply URA.wf_mon; et. }
     { eapply H0; et. eapply URA.wf_mon; et. rewrite URA.add_comm. et. }
   Qed.
 
   Lemma Emp_Sepconj_l: ∀ P : iProp, Entails P (Sepconj Emp P).
   Proof.
-    ii. econs. ii. exists ε, r. splits; ss. rewrite URA.unit_idl. et.
+    ii. uipropall. ii. exists ε, r. splits; ss. rewrite URA.unit_idl. et.
   Qed.
 
   Lemma Emp_Sepconj_r: ∀ P : iProp, Entails (Sepconj Emp P) P.
   Proof.
-    ii. econs. ii. inv H. des; subst. inv H1. rewrite URA.unit_idl. et.
+    ii. uipropall. ii. inv H. des; subst. rewrite URA.unit_idl. et.
   Qed.
 
   Lemma Sepconj_comm: ∀ P Q : iProp, Entails (Sepconj P Q) (Sepconj Q P).
   Proof.
-    ii. econs. ii. unfold Sepconj in *. des. subst. exists b, a. splits; et. apply URA.add_comm.
+    ii. uipropall. ii. unfold Sepconj in *. des. subst. exists b, a. splits; et. apply URA.add_comm.
   Qed.
 
   Lemma Sepconj_assoc: ∀ P Q R : iProp, Entails (Sepconj (Sepconj P Q) R) (Sepconj P (Sepconj Q R)).
   Proof.
-    ii. econs. ii. unfold Sepconj in *. des; subst. esplits; [|apply H2| |apply H3|apply H1]; ss.
+    ii. uipropall. ii. unfold Sepconj in *. des; subst. esplits; [|apply H2| |apply H3|apply H1]; ss.
     rewrite URA.add_assoc. ss.
   Qed.
 
   Lemma Wand_intro_r: ∀ P Q R : iProp, Entails (Sepconj P Q) R → Entails P (Wand Q R).
   Proof.
-    ii. econs. ii. eapply H; et. exists r, rp. splits; et.
+    ii. uipropall. ii. eapply H; et.
   Qed.
 
   Lemma Wand_elim_l: ∀ P Q R : iProp, Entails P (Wand Q R) → Entails (Sepconj P Q) R.
   Proof.
-    ii. econs. ii. unfold Sepconj in *. des; subst. eapply H; et. eapply URA.wf_mon; et.
+    ii. uipropall. ii. unfold Sepconj in *. des; subst. eapply H; et. eapply URA.wf_mon; et.
   Qed.
 
   Lemma Upd_intro: ∀ P : iProp, Entails P (Upd P).
   Proof.
-    ii. econs. ii. exists r. splits; auto.
+    ii. uipropall. ii. exists r. splits; auto.
   Qed.
 
   Lemma Upd_mono: ∀ P Q : iProp, Entails P Q -> Entails (Upd P) (Upd Q).
   Proof.
-    ii. econs. ii. exploit H0; et. i. des.
+    ii. uipropall. ii. exploit H0; et. i. des.
     exploit (H r1); et. eapply URA.wf_mon; et.
   Qed.
 
   Lemma Upd_trans: ∀ P : iProp, Entails (Upd (Upd P)) (Upd P).
   Proof.
-    ii. econs. ii. exploit H; et. i. des. exploit x0; eauto.
+    ii. uipropall. ii. exploit H; et. i. des. exploit x0; eauto.
   Qed.
 
   Lemma Upd_frame_r: ∀ P R : iProp, Entails (Sepconj (Upd P) R) (Upd (Sepconj P R)).
   Proof.
-    ii. econs. ii. unfold Sepconj in *. des. subst. exploit (H1 (b ⋅ ctx)); et.
+    ii. uipropall. ii. unfold Sepconj in *. des. subst. exploit (H1 (b ⋅ ctx)); et.
     { rewrite URA.add_assoc. et. }
     i. des. esplits; [..|eapply x1|eapply H2]; ss.
     rewrite <- URA.add_assoc. et.
@@ -223,120 +263,117 @@ Section IRIS.
 
   Lemma iProp_bi_mixin:
     BiMixin
-      Entails2 Emp Pure And Or Impl
+      Entails Emp Pure And Or Impl
       (@Univ) (@Ex) Sepconj Wand
       Persistently.
   Proof.
-  Admitted.
-  (*   econs. *)
-  (*   - exact PreOrder_Entails. *)
-  (*   - econs. *)
-  (*     { ii. split; econs; ii; eapply H; et. } *)
-  (*     { split. des. i. split; i. *)
-  (*       { eapply H; et. } *)
-  (*       { eapply H0; et. } *)
-  (*     } *)
-  (*   - econs. i. split. *)
-  (*     { ii. eapply H. ss. } *)
-  (*     { ii. eapply H. ss. } *)
-  (*   - econs. i. split. *)
-  (*     { ii. inv H2. split. *)
-  (*       { eapply H; et. } *)
-  (*       { eapply H0; et. } *)
-  (*     } *)
-  (*     { ii. inv H2. split. *)
-  (*       { eapply H; et. } *)
-  (*       { eapply H0; et. } *)
-  (*     } *)
-  (*   - econs. i. split. *)
-  (*     { ii. inv H2. *)
-  (*       { left. eapply H; et. } *)
-  (*       { right. eapply H0; et. } *)
-  (*     } *)
-  (*     { ii. inv H2. *)
-  (*       { left. eapply H; et. } *)
-  (*       { right. eapply H0; et. } *)
-  (*     } *)
-  (*   - econs. i. split. *)
-  (*     { ii. eapply H0; et. eapply H2; et. eapply H; et. } *)
-  (*     { ii. eapply H0; et. eapply H2; et. eapply H; et. } *)
-  (*   - econs. i. split. *)
-  (*     { ii. exploit H; et. i. eapply x2; et. } *)
-  (*     { ii. exploit H; et. i. eapply x2; et. } *)
-  (*   - econs. i. split. *)
-  (*     { ii. inv H1. exploit H; et. i. eexists. eapply x2; et. } *)
-  (*     { ii. inv H1. exploit H; et. i. eexists. eapply x2; et. } *)
-  (*   - econs. i. split. *)
-  (*     { ii. inv H2. des. subst. eexists. esplits; eauto. *)
-  (*       { eapply H; et. eapply URA.wf_mon; et. } *)
-  (*       { eapply H0; et. eapply URA.wf_mon; et. rewrite URA.add_comm. et. } *)
-  (*     } *)
-  (*     { ii. inv H2. des. subst. eexists. esplits; eauto. *)
-  (*       { eapply H; et. eapply URA.wf_mon; et. } *)
-  (*       { eapply H0; et. eapply URA.wf_mon; et. rewrite URA.add_comm. et. } *)
-  (*     } *)
-  (*   - econs. i. split. *)
-  (*     { ii. exploit H2; et. *)
-  (*       { eapply H; et. eapply URA.wf_mon; et. rewrite URA.add_comm. et. } *)
-  (*       { i. eapply H0; et. } *)
-  (*     } *)
-  (*     { ii. exploit H2; et. *)
-  (*       { eapply H; et. eapply URA.wf_mon; et. rewrite URA.add_comm. et. } *)
-  (*       { i. eapply H0; et. } *)
-  (*     } *)
-  (*   - ii. econs. i. split. *)
-  (*     { ii. eapply H; ss. eapply URA.wf_unit. } *)
-  (*     { ii. eapply H; ss. eapply URA.wf_unit. } *)
-  (*   - exact Pure_intro. *)
-  (*   - exact Pure_elim. *)
-  (*   - exact And_elim_l. *)
-  (*   - exact And_elim_r. *)
-  (*   - exact And_intro. *)
-  (*   - exact Or_intro_l. *)
-  (*   - exact Or_intro_r. *)
-  (*   - exact Or_elim. *)
-  (*   - exact Impl_intro_r. *)
-  (*   - exact Impl_elim_l. *)
-  (*   - exact Univ_intro. *)
-  (*   - exact Univ_elim. *)
-  (*   - exact Ex_intro. *)
-  (*   - exact Ex_elim. *)
-  (*   - exact Sepconj_mono. *)
-  (*   - exact Emp_Sepconj_l. *)
-  (*   - exact Emp_Sepconj_r. *)
-  (*   - exact Sepconj_comm. *)
-  (*   - exact Sepconj_assoc. *)
-  (*   - exact Wand_intro_r. *)
-  (*   - exact Wand_elim_l. *)
-  (*   - ii. econs; ii. eapply H; et. eapply URA.wf_unit. *)
-  (*   - ii. econs; ii. eapply H; et. *)
-  (*   - ii. econs; ii. red in H. subst. ss. *)
-  (*   - ii. econs; ii. eapply H; et. *)
-  (*   - ii. econs; ii. inv H. exists x. ss. *)
-  (*   - ii. econs; ii. unfold Sepconj in *. des; subst. ss. *)
-  (*   - ii. econs; ii. inv H. unfold Sepconj in *. esplits; et. rewrite URA.unit_idl. et. *)
-  (* Qed. *)
+    econs.
+    - exact PreOrder_Entails.
+    - econs.
+      { uipropall. ii. split; ii; eapply H; et. }
+      { uipropall. i. econs. i. des. split; i.
+        { eapply H; et. }
+        { eapply H1; et. }
+      }
+    - econs. i. split.
+      { uipropall. ii. eapply H. ss. }
+      { uipropall. ii. eapply H. ss. }
+    - econs. i. split.
+      { uipropall. ii. inv H2. split.
+        { eapply H; et. }
+        { eapply H0; et. }
+      }
+      { uipropall. ii. inv H2. split.
+        { eapply H; et. }
+        { eapply H0; et. }
+      }
+    - econs. i. split.
+      { uipropall. ii. inv H2.
+        { left. eapply H; et. }
+        { right. eapply H0; et. }
+      }
+      { uipropall. ii. inv H2.
+        { left. eapply H; et. }
+        { right. eapply H0; et. }
+      }
+    - econs. i. split.
+      { uipropall. ii. eapply H0; et. eapply H2; et. eapply H; et. }
+      { uipropall. ii. eapply H0; et. eapply H2; et. eapply H; et. }
+    - econs. i. split.
+      { uipropall. ii. exploit H; et. i. eapply x2; et. }
+      { uipropall. ii. exploit H; et. i. eapply x2; et. }
+    - econs. i. split.
+      { uipropall. ii. inv H1. exploit H; et. i. eexists. eapply x2; et. }
+      { uipropall. ii. inv H1. exploit H; et. i. eexists. eapply x2; et. }
+    - econs. i. split.
+      { uipropall. ii. inv H2. des. subst. eexists. esplits; eauto.
+        { eapply H; et. eapply URA.wf_mon; et. }
+        { eapply H0; et. eapply URA.wf_mon; et. rewrite URA.add_comm. et. }
+      }
+      { uipropall. ii. inv H2. des. subst. eexists. esplits; eauto.
+        { eapply H; et. eapply URA.wf_mon; et. }
+        { eapply H0; et. eapply URA.wf_mon; et. rewrite URA.add_comm. et. }
+      }
+    - econs. uipropall. i. split.
+      { ii. exploit H2; et.
+        { eapply H; et. eapply URA.wf_mon; et. rewrite URA.add_comm. et. }
+        { i. eapply H0; et. }
+      }
+      { ii. exploit H2; et.
+        { eapply H; et. eapply URA.wf_mon; et. rewrite URA.add_comm. et. }
+        { i. eapply H0; et. }
+      }
+    - ii. econs. uipropall. i. split.
+      { ii. eapply H; ss. eapply URA.wf_unit. }
+      { ii. eapply H; ss. eapply URA.wf_unit. }
+    - exact Pure_intro.
+    - exact Pure_elim.
+    - exact And_elim_l.
+    - exact And_elim_r.
+    - exact And_intro.
+    - exact Or_intro_l.
+    - exact Or_intro_r.
+    - exact Or_elim.
+    - exact Impl_intro_r.
+    - exact Impl_elim_l.
+    - exact Univ_intro.
+    - exact Univ_elim.
+    - exact Ex_intro.
+    - exact Ex_elim.
+    - exact Sepconj_mono.
+    - exact Emp_Sepconj_l.
+    - exact Emp_Sepconj_r.
+    - exact Sepconj_comm.
+    - exact Sepconj_assoc.
+    - exact Wand_intro_r.
+    - exact Wand_elim_l.
+    - ii. uipropall. i. eapply H; et. eapply URA.wf_unit.
+    - ii. uipropall. i. eapply H; et.
+    - ii. uipropall. ii. subst. ss.
+    - ii. uipropall. ii. specialize (H x). uipropall. eapply H; et.
+    - ii. uipropall. i. des. eexists. uipropall. et.
+    - ii. uipropall. i. des. subst. ss.
+    - ii. uipropall. ii. inv H. esplits; et. rewrite URA.unit_idl. et.
+  Qed.
 
   Lemma iProp_bi_later_mixin:
     BiLaterMixin
-      Entails2 Pure Or Impl
+      Entails Pure Or Impl
       (@Univ) (@Ex) Sepconj Persistently Later.
   Proof.
-  Admitted.
-  (*   econs. *)
-  (*   - ii. econs. i. split. *)
-  (*     { i. eapply H; et. } *)
-  (*     { i. eapply H; et. } *)
-  (*   - ii. eapply H; et. *)
-  (*   - ii. ss. *)
-  (*   - ii. econs; ii. eapply H. *)
-  (*   - ii. econs; ii. right. ss. *)
-  (*   - ii. ss. *)
-  (*   - ii. ss. *)
-  (*   - ii. ss. *)
-  (*   - ii. ss. *)
-  (*   - ii. econs; ii. right. ss. *)
-  (* Qed. *)
+    econs.
+    - ii. uipropall. i. split.
+      { i. eapply H; et. }
+    - ii. uipropall. eapply H; et.
+    - ii. uipropall. ss.
+    - ii. uipropall. ii. specialize (H x). uipropall. eapply H.
+    - ii. uipropall. ii. right. des. exists x. uipropall. ss.
+    - ii. uipropall. ss.
+    - ii. uipropall. ss.
+    - ii. uipropall. ss.
+    - ii. uipropall. ss.
+    - ii. uipropall. ii. right. ss.
+  Qed.
 
   Canonical Structure iPropI: bi :=
     {| bi_bi_mixin := iProp_bi_mixin;
@@ -345,299 +382,52 @@ Section IRIS.
   (** extra BI instances *)
   Lemma iProp_bupd_mixin: BiBUpdMixin iPropI Upd.
   Proof.
-  Admitted.
-  (*   econs. *)
-  (*   - ii. econs. i. split. *)
-  (*     { ii. exploit H1; eauto. i. des. esplits; eauto. *)
-  (*       eapply H; et. eapply URA.wf_mon; et. } *)
-  (*     { ii. exploit H1; eauto. i. des. esplits; eauto. *)
-  (*       eapply H; et. eapply URA.wf_mon; et. } *)
-  (*   - exact Upd_intro. *)
-  (*   - exact Upd_mono. *)
-  (*   - exact Upd_trans. *)
-  (*   - exact Upd_frame_r. *)
-  (* Qed. *)
+    econs.
+    - ii. econs. unfold bupd. uipropall. i. split.
+      { ii. exploit H1; eauto. i. des. esplits; eauto.
+        eapply H; et. eapply URA.wf_mon; et. }
+      { ii. exploit H1; eauto. i. des. esplits; eauto.
+        eapply H; et. eapply URA.wf_mon; et. }
+    - exact Upd_intro.
+    - exact Upd_mono.
+    - exact Upd_trans.
+    - exact Upd_frame_r.
+  Qed.
   Global Instance iProp_bi_bupd: BiBUpd iPropI := {| bi_bupd_mixin := iProp_bupd_mixin |}.
 
   Global Instance iProp_bupd_absorbing (P: iPropI): Absorbing (bupd P).
   Proof.
-  Admitted.
-  (*   ii. econs; ii. red in H. inv H. des. subst. exploit H3; et. *)
-  (*   eapply URA.wf_mon. rewrite URA.add_comm. rewrite URA.add_assoc. et. *)
-  (* Qed. *)
+    ii. repeat red. unfold bupd, bi_bupd_bupd in *. ss. uipropall.
+    ii. repeat red in H. uipropall. des. subst. exploit H2; et.
+    eapply URA.wf_mon. rewrite URA.add_comm. rewrite URA.add_assoc. et.
+  Qed.
 
   Global Instance iProp_pure_forall: BiPureForall iPropI.
   Proof.
-  Admitted.
-  (*   ii. econs; ii. eapply H. *)
-  (* Qed. *)
+    ii. red. red. uipropall. ii. red. red in H.
+    uipropall. i. specialize (H a). red in H. uipropall. ss.
+  Qed.
+
+End IRIS.
+
+Hint Rewrite (Seal.sealing_eq "iProp"): iprop.
+#[export] Hint Unfold Sepconj Pure Ex Univ Own And Or Impl Wand Emp Persistently Later Upd Entails: iprop.
+
+From iris.proofmode Require Export tactics.
 
 
-  From iris.proofmode Require Export tactics class_instances.
+Section TEST.
+  Context {Σ: GRA.t}.
 
-  (** AsEmpValid *)
-  Global Instance as_emp_valid_emp_valid (P: iPropI) : AsEmpValid0 (⊢ P) P | 0.
-  Proof. by rewrite /AsEmpValid. Qed.
-  Global Instance as_emp_valid_entails (P Q: iPropI) : AsEmpValid0 (P ⊢ Q) (P -∗ Q).
-  Proof. split; [ apply bi.entails_wand | apply bi.wand_entails ]. Qed.
-  Global Instance as_emp_valid_equiv (P Q: iPropI) : AsEmpValid0 (P ≡ Q) (P ∗-∗ Q).
-  Proof. Admitted.
+  Goal forall (P Q R: iPropI) (PQ: P -∗ Q) (QR: Q -∗ R), P -∗ R.
+  Proof.
+    i. iStartProof. iIntros "H".
+    iApply QR. iApply PQ. iApply "H".
+  Qed.
 
-  Goal forall (P Q: iPropI), bi_entails (bi_sep (bupd P) Q) (bupd Q).
+  Goal forall (P Q: iPropI), ((bupd P) ∗ Q) -∗ (bupd Q).
   Proof.
     i. iStartProof.
     iIntros "[Hxs Hys]". iMod "Hxs". iApply "Hys".
   Qed.
-
-  Variable P Q R: iProp.
-  Hypothesis PQ: bi_entails P Q.
-  Hypothesis QR: bi_entails Q R.
-
-
-  From stdpp Require Import namespaces hlist pretty.
-  From iris.bi Require Export bi telescopes.
-  From iris.proofmode Require Import base intro_patterns spec_patterns
-       sel_patterns coq_tactics reduction.
-  From iris.proofmode Require Export classes notation.
-  From iris.prelude Require Import options.
-  Export ident.
-
-  From iris.proofmode Require Import tactics ltac_tactics.
-
-
-  Local Ltac iApplyHypExact H :=
-    eapply tac_assumption with H _ _; (* (i:=H) *)
-    [pm_reflexivity
-    |iSolveTC
-    |pm_reduce; iSolveTC ||
-                         fail 1 "iApply: remaining hypotheses not affine and the goal not absorbing"].
-
-  Local Ltac iApplyHypLoop H :=
-    first
-      [eapply tac_apply with H _ _ _;
-       [pm_reflexivity
-       |iSolveTC
-       |pm_reduce;
-        pm_prettify (* reduce redexes created by instantiation *)]].
-
-  Tactic Notation "iApplyHyp" constr(H) :=
-    first
-      [iApplyHypExact H
-      |iApplyHypLoop H
-      |lazymatch iTypeOf H with
-       | Some (_,?Q) => fail 1 "iApply: cannot apply" Q
-       end].
-
-  Tactic Notation "iApply" open_constr(lem) :=
-    iPoseProofCore lem as false (fun H => iApplyHyp H).
-
-
-  Tactic Notation "iPoseProofCoreHyp" constr(H) "as" constr(Hnew) :=
-    let Δ := iGetCtx in
-    notypeclasses refine (tac_pose_proof_hyp _ H Hnew _ _);
-    pm_reduce;
-    lazymatch goal with
-    | |- False =>
-      let lookup := pm_eval (envs_lookup_delete false H Δ) in
-      lazymatch lookup with
-      | None =>
-        let H := pretty_ident H in
-        fail "iPoseProof:" H "not found"
-      | _ =>
-        let Hnew := pretty_ident Hnew in
-        fail "iPoseProof:" Hnew "not fresh"
-      end
-    | _ => idtac
-    end.
-
-  Tactic Notation "iPoseProofCoreLem" open_constr(lem) "as" tactic3(tac) :=
-    let Hnew := iFresh in
-    notypeclasses refine (tac_pose_proof _ Hnew _ _ (into_emp_valid_proj _ _ _ lem) _);
-    [iIntoEmpValid
-    |pm_reduce;
-     lazymatch goal with
-     | |- False =>
-       let Hnew := pretty_ident Hnew in
-       fail "iPoseProof:" Hnew "not fresh"
-     | _ => tac Hnew
-     end];
-    (* Solve all remaining TC premises generated by [iIntoEmpValid] *)
-    try iSolveTC.
-
-  Tactic Notation "iPoseProofCore" open_constr(lem)
-         "as" constr(p) tactic3(tac) :=
-    iStartProof;
-    let t := lazymatch lem with ITrm ?t ?xs ?pat => t | _ => lem end in
-    let t := lazymatch type of t with string => constr:(INamed t) | _ => t end in
-    let spec_tac Htmp :=
-        lazymatch lem with
-        | ITrm _ ?xs ?pat => iSpecializeCore (ITrm Htmp xs pat) as p
-        | _ => idtac
-        end in
-    pose t
-  .
-    (* lazymatch type of t with *)
-    (* | _ => iPoseProofCoreLem t as (fun Htmp => spec_tac Htmp; [..|tac Htmp]) *)
-    (* end. *)
-
-
-
-  Ltac iIntoEmpValid_go := first
-                             [(* Case [φ → ψ] *)
-                               notypeclasses refine (into_emp_valid_impl _ _ _ _ _);
-                               [(*goal for [φ] *)|iIntoEmpValid_go]
-                              |(* Case [∀ x : A, φ] *)
-                              notypeclasses refine (into_emp_valid_forall _ _ _ _); iIntoEmpValid_go
-                              |(* Case [∀.. x : TT, φ] *)
-                              notypeclasses refine (into_emp_valid_tforall _ _ _ _); iIntoEmpValid_go
-                              |(* Case [P ⊢ Q], [P ⊣⊢ Q], [⊢ P] *)
-                              notypeclasses refine (into_emp_valid_here _ _ _)].
-
-  Ltac iIntoEmpValid :=
-    (* Factor out the base case of the loop to avoid needless backtracking *)
-    iIntoEmpValid_go;
-    [.. (* goals for premises *)
-    |iSolveTC ||
-              let φ := lazymatch goal with |- AsEmpValid ?φ _ => φ end in
-              fail "iPoseProof:" φ "not a BI assertion"].
-
-
-  Goal bi_entails P R.
-  Proof.
-    i. iStartProof. iIntros "H". iApply QR.
-    Show Proof.
-    Set Printing All.
-
-    let Hnew := iFresh in
-    notypeclasses refine (tac_pose_proof _ Hnew _ _ (into_emp_valid_proj _ _ _ QR) _).
-    {
-
-
-      refine (@into_emp_valid_forall _ _ _ _ _ _).
-
-      iIntoEmpValid_go.
-
-      Local Opaque bi_entails.
-      refine (into_emp_valid_forall _ _ _ _).
-
-      @into_emp_valid_forall ?PROP ?A
-        : forall (φ : forall _ : ?A, Type) (P0 : bi_car ?PROP) (x : ?A) (_ : @IntoEmpValid ?PROP (φ x) P0),
-          @IntoEmpValid ?PROP (forall x0 : ?A, φ x0) P0
-      where
-      ?PROP : [Σ : GRA.t  P : iProp  Q : iProp  R : iProp  PQ : @bi_entails iPropI P Q  QR : @bi_entails iPropI Q R
-               |- bi]
-                ?A : [Σ : GRA.t  P : iProp  Q : iProp  R : iProp  PQ : @bi_entails iPropI P Q  QR : @bi_entails iPropI Q R
-                      |- Type]
-
-
-      iIntoEmpValid_go.
-
-    ].
-
-
-      notypeclasses refine (into_emp_valid_here _ _ _).
-
-
-      first
-        [(* Case [φ → ψ] *)
-          notypeclasses refine (into_emp_valid_impl _ _ _ _ _);
-          [(*goal for [φ] *)|iIntoEmpValid_go]
-         |(* Case [∀ x : A, φ] *)
-         notypeclasses refine (into_emp_valid_forall _ _ _ _); iIntoEmpValid_go
-         |(* Case [∀.. x : TT, φ] *)
-         notypeclasses refine (into_emp_valid_tforall _ _ _ _); iIntoEmpValid_go
-         |(* Case [P ⊢ Q], [P ⊣⊢ Q], [⊢ P] *)
-         notypeclasses refine (into_emp_valid_here _ _ _)].
-
-
-      iIntoEmpValid_go.
-
-      ; cycle 2.
-      { eapply class_instances.as_emp_valid_entails.
-        eapply as_emp_valid_entails.
-
-
-        eapply as_emp_valid_entails.
-        {
-
-        red.        typeclasses eauto.
-
-        solve [ once typeclasses eauto ].
-        .
-        iSolveTC.
-
-      3:{ iSolveTC.
-        [.. (* goals for premises *)
-        |iSolveTC ||
-                  let φ := lazymatch goal with |- AsEmpValid ?φ _ => φ end in
-                  fail "iPoseProof:" φ "not a BI assertion"].
-
-      iIntoEmpValid.
-
-
-
-
-      let Hnew := iFresh in
-      notypeclasses refine (tac_pose_proof _ Hnew _ _ (into_emp_valid_proj _ _ _ QR) _).
-
-      [iIntoEmpValid
-      |pm_reduce;
-       lazymatch goal with
-       | |- False =>
-         let Hnew := pretty_ident Hnew in
-         fail "iPoseProof:" Hnew "not fresh"
-       | _ => iApplyHyp Hnew
-       end];
-      (* Solve all remaining TC premises generated by [iIntoEmpValid] *)
-      try iSolveTC.
-
-
-    iPoseProofCoreLem QR as (fun Htmp => iApplyHyp Htmp).
-
-
-
-
-    end.
-
-
-    iStartProof;
-      let t := lazymatch QR with ITrm ?t ?xs ?pat => t | _ => QR end in
-      let t := lazymatch type of t with string => constr:(INamed t) | _ => t end in
-      let spec_tac Htmp :=
-          lazymatch QR with
-          | ITrm _ ?xs ?pat => iSpecializeCore (ITrm Htmp xs pat) as false
-          | _ => idtac
-          end in
-      lazymatch type of QR with
-      | _ => iPoseProofCoreLem QR as (fun Htmp => idtac Htmp; [..|iApplyHyp Htmp])
-      end.
-
-
-    iApply QR. iApply H. iApply H0. iApply H in "H".
-
-    iIntros "[Hxs Hys]". iMod "Hys". iApply "Hxs".
-  Qed.
-
-End IRIS.
-
-From iris.proofmode Require Export tactics.
-
-Section IRIS.
-  Context {Σ: GRA.t}.
-
-  Variable P Q R: iPropI.
-  Hypothesis PQ: bi_entails P Q.
-  Hypothesis QR: bi_entails Q R.
-
-  Goal bi_entails P R.
-  Proof.
-    i. iStartProof. iIntros "H".
-    Set Printing All.
-    iApply QR. iApply H. iApply H0. iApply H in "H".
-
-    iIntros "[Hxs Hys]". iMod "Hys". iApply "Hxs".
-  Qed.
-
-
-
-End IRIS.
+End TEST.
